Second wave of fixes after merge.

TransVal/SMT.v
@@ -1,5 +1,5 @@
 Require Import List EqNat Bool.
-Require Import IL Exp Val bitvec DecSolve.
+Require Import IL BitVector Exp MoreExp SetOperations Val DecSolve.
 
 Set Implicit Arguments.
 
@@ -208,8 +208,96 @@ Proof.
     simpl. rewrite H. split; eauto.
 Qed.
 
-  (*
-  *** Local Variables: ***
-  *** coq-load-path: (("../" "Lvc")) ***
-  *** End: ***
-  *)
+Fixpoint freeVars (s:smt) :=
+match s with
+| funcApp f x => list_union (List.map (Exp.freeVars) x)
+| smtAnd a b => freeVars a ∪ freeVars b
+| smtOr a b => freeVars a ∪ freeVars b
+| smtNeg a => freeVars a
+| ite c t f => freeVars t ∪ freeVars f ∪ Exp.freeVars c
+| smtImp a b => freeVars a ∪ freeVars b
+| smtFalse => {}
+| smtTrue =>  {}
+|constr e1 e2 => Exp.freeVars e1 ∪ Exp.freeVars e2
+end.
+
+Lemma models_agree F E E' s:
+  agree_on eq (freeVars s) E E'
+  -> (models F E s <-> models F E' s).
+
+Proof.
+intros agree; general  induction s; simpl in *; try reflexivity.
+- rewrite (IHs1 F E E'), (IHs2 F E E'); eauto with cset. reflexivity.
+- rewrite (IHs1 F E E'), (IHs2 F E E'); eauto with cset. reflexivity.
+- rewrite (IHs F E E'); eauto with cset. reflexivity.
+- assert (agree_on eq (Exp.freeVars e) E E') by eauto with cset.
+  assert (exp_eval (to_partial E) e = exp_eval (to_partial E') e). {
+    eapply exp_eval_agree; symmetry; eauto.
+    eapply agree_on_partial; eauto.
+  }
+ unfold smt_eval in *.
+  case_eq (exp_eval (to_partial E) e); intros.
+  +  rewrite <- H0. rewrite H1. case_eq(val2bool v); intros.
+     * rewrite (IHs1 F E E'); eauto with cset.
+     * rewrite (IHs2 F E E'); eauto with cset.
+  + rewrite <- H0; rewrite H1. case_eq (val2bool undef_substitute); intros.
+    * rewrite (IHs1 F E E'); eauto with cset.
+    * rewrite (IHs2 F E E'); eauto with cset.
+- rewrite (IHs1 F E E'), (IHs2 F E E'); eauto with cset. reflexivity.
+- assert (exp_eval (to_partial E) e = exp_eval (to_partial E') e). {
+    eapply exp_eval_agree; symmetry; eauto.
+    eapply agree_on_partial. eapply agree_on_incl; eauto.  }
+  assert (exp_eval (to_partial E) e0 = exp_eval (to_partial E') e0). {
+    eapply exp_eval_agree; symmetry; eauto.
+    eapply agree_on_partial. eapply agree_on_incl; eauto.  }
+  unfold smt_eval in *.
+  rewrite <- H; rewrite <- H0.
+  unfold val2bool.
+  case_eq (exp_eval (to_partial E) e); case_eq (exp_eval (to_partial E) e0); intros;
+  try rewrite bvEq_equiv_eq; reflexivity.
+- destruct p.
+  assert (List.map (smt_eval E) a =List.map (smt_eval E') a).
+  + general induction a.
+    * eauto.
+    * simpl.
+      assert (smt_eval E a = smt_eval E' a).
+      { unfold smt_eval.
+      pose proof (exp_eval_agree (E:=to_partial E) (E':=to_partial E') a (v:=exp_eval (to_partial E) a)).
+      rewrite H; eauto.
+      eapply agree_on_partial.
+      simpl in agree.
+      eapply (agree_on_incl (bv:=Exp.freeVars a)(lv:=list_union (Exp.freeVars a:: List.map Exp.freeVars a0))); eauto.
+      cset_tac; simpl.
+      eapply list_union_start_swap.
+      cset_tac; eauto. }
+      { rewrite H. f_equal. eapply IHa; eauto.
+        eapply (agree_on_incl (bv:=list_union (List.map Exp.freeVars a0))
+               (lv:=list_union (List.map Exp.freeVars (a::a0)))); eauto.
+        cset_tac; simpl.
+        eapply list_union_start_swap.
+        eapply union_right; eauto. }
+  + rewrite H.  split; eauto.
+Qed.
+
+Lemma exp_freeVars_list_agree (E: onv val) e el:
+    (forall x, x ∈ list_union (Exp.freeVars e:: List.map Exp.freeVars el) -> exists v, E x = Some v)
+    ->(forall x, x ∈ Exp.freeVars e -> (exists v, E x = Some v)) /\
+      (forall x, x ∈ list_union (List.map Exp.freeVars el) -> exists v, E x = Some v).
+
+Proof.
+  intros. split;
+  intros; specialize (H x); destruct H; eauto;
+    simpl;
+    eapply list_union_start_swap;
+    cset_tac; eauto.
+Qed.
+
+Lemma exp_freeVars_bin_agree (E:onv val) a b:
+  (forall x, x ∈ (union (Exp.freeVars a) (Exp.freeVars b)) -> exists v, E x = Some v)
+    ->(forall x, x ∈ Exp.freeVars a -> (exists v, E x = Some v)) /\
+      (forall x, x ∈ Exp.freeVars b -> exists v, E x = Some v).
+
+Proof.
+  intros.
+  split; intros; specialize (H x); destruct H; cset_tac; eauto.
+Qed.
