TransVal/CombineEnv.v
@@ -1,27 +1,24 @@
 Require Import List Arith.
 Require Import IL Annotation AutoIndTac Exp MoreExp RenamedApart Fresh Util.
 Require Import SetOperations Sim Var.
-Require Import bitvec smt nofun freeVars.
-Require Import Compute Guards ILFtoSMT tvalTactics TUtil GuardProps ComputeProps.
+Require Import SMT NoFun.
+Require Import Guards ILFtoSMT GuardProps ComputeProps.
 
 (** Definitons **)
 Definition combineEnv D (E1:onv val) E2 :=
-fun x => if [x ∈ D] then E1 x else E2 x.
+  fun x => if [x ∈ D] then E1 x else E2 x.
 
 (** Lemmata **)
 
-Lemma combineenv_agree D E E':
-  agree_on eq D (combineEnv D E E') E.
-
+Lemma combineenv_agree D E E'
+  : agree_on eq D (combineEnv D E E') E.
 Proof.
   hnf; intros. unfold combineEnv. cases; eauto; isabsurd.
 Qed.
 
-Lemma exp_combineenv_eql:
-forall e D Es Et v,
-Exp.freeVars e ⊆ D
--> (exp_eval (combineEnv D Es Et) e= v <-> exp_eval Es e = v).
-
+Lemma exp_combineenv_eql e D Es Et v
+  : Exp.freeVars e ⊆ D
+    -> (exp_eval (combineEnv D Es Et) e = v <-> exp_eval Es e = v).
 Proof.
   intros. split; intros.
   - eapply (exp_eval_agree (E:=(combineEnv D Es Et))); eauto.
@@ -33,25 +30,20 @@ Proof.
     symmetry. eapply combineenv_agree.
 Qed.
 
-  Lemma explist_combineenv_eql:
-forall el D Es Et rl,
-list_union (List.map Exp.freeVars el) ⊆ D
--> ( omap (exp_eval (combineEnv D Es Et)) el = rl <-> omap (exp_eval Es) el = rl).
-
+Lemma explist_combineenv_eql el D Es Et rl
+  : list_union (List.map Exp.freeVars el) ⊆ D
+    -> ( omap (exp_eval (combineEnv D Es Et)) el = rl <-> omap (exp_eval Es) el = rl).
 Proof.
-  intros; split; intros.
-  - general induction el; eauto.
-    + simpl. simpl in H. hnf in H.
-      pose proof (exp_combineenv_eql a D Es Et (exp_eval (combineEnv D Es Et) a)); eauto.
-      destruct H0; hnf; intros; try setSubstUnion H.
-      * rewrite H0; eauto. erewrite IHel ; eauto.
-        hnf; intros. setSubstUnion H.
-  - general induction el; eauto.
-    + simpl; simpl in H; hnf in H.
-      pose proof (exp_combineenv_eql a D Es Et (exp_eval (combineEnv D Es Et) a)); eauto.
-      destruct H0; hnf; intros; try setSubstUnion H.
-      * rewrite H0; eauto. erewrite IHel; eauto.
-        hnf; intros; setSubstUnion H.
+  intros.
+  general induction el; simpl in * |- *; eauto.
+  - reflexivity.
+  - rewrite list_union_start_swap in H.
+    pose proof (exp_combineenv_eql a D Es Et (exp_eval (combineEnv D Es Et) a));
+      eauto.
+      destruct H0; [ hnf; intros; eauto with cset | ].
+    * rewrite H0; eauto.
+      edestruct (IHel D Es Et); [ hnf; intros; eauto with cset| ].
+      erewrite H3; eauto. reflexivity.
 Qed.
 
 Lemma combineenv_eql:
@@ -168,18 +160,15 @@ Lemma combineenv_eqr:
     -> (models F (to_total Et) s <-> models F (to_total (combineEnv D Es Et)) s).
 
 Proof.
-  intros.  general induction s; try reflexivity; simpl.
-  - rewrite (IHs1 F D Es Et). rewrite (IHs2 F D Es Et).
-    + reflexivity.
-    + setSubst2 H.
-    + setSubst2 H.
-  - rewrite (IHs1 F D Es Et).  rewrite (IHs2 F D Es Et).
-    + reflexivity.
-    + setSubst2 H.
-    + setSubst2 H.
-  - rewrite (IHs F D Es Et).
-    + reflexivity.
-    + setSubst2 H.
+  intros.  general induction s; try reflexivity; simpl in * |- *.
+  - rewrite (IHs1 F D Es Et); eauto with cset.
+    rewrite (IHs2 F D Es Et); eauto with cset.
+    reflexivity.
+  - rewrite (IHs1 F D Es Et); eauto with cset.
+    rewrite (IHs2 F D Es Et); eauto with cset.
+    reflexivity.
+  - rewrite (IHs F D Es Et); eauto with cset.
+    reflexivity.
   - case_eq (exp_eval (to_partial (to_total (combineEnv D Es Et))) e); intros.
     + pose proof (exp_combineenv_eqr' e D Es Et (Some v)).
       assert (agree_on eq (Exp.freeVars e ∩ D) Es Et).
@@ -188,28 +177,25 @@ Proof.
         specialize (H1 H0).
         unfold smt_eval; rewrite H1.
         case_eq (val2bool v); intros.
-        { rewrite (IHs1 F D Es Et).
-          - rewrite H0, H4. reflexivity.
-          - setSubst2 H. }
-        { rewrite (IHs2 F D Es Et).
-          - rewrite H0, H4. reflexivity.
-          - setSubst2 H. }
+        { rewrite (IHs1 F D Es Et); eauto with cset.
+          rewrite H0, H4. reflexivity.
+        }
+        { rewrite (IHs2 F D Es Et); eauto with cset.
+          rewrite H0, H4. reflexivity.
+        }
      + pose proof (exp_combineenv_eqr' e D Es Et None).
        assert (agree_on eq (Exp.freeVars e ∩ D) Es Et).
        * hnf; intros. hnf in H. simpl in H. cset_tac.
        * destruct H1; eauto.  specialize (H1 H0).
          unfold smt_eval; rewrite H0, H1.
          case_eq (val2bool undef_substitute); intros.
-         { rewrite (IHs1 F D Es Et).
-           - reflexivity.
-           - setSubst2 H. }
-         { rewrite (IHs2 F D Es Et).
-           - reflexivity.
-           - setSubst2 H. }
-  - rewrite (IHs1 F D Es Et).  rewrite (IHs2 F D Es Et).
-    + reflexivity.
-    + setSubst2 H.
-    + setSubst2 H.
+         { rewrite (IHs1 F D Es Et); eauto with cset.
+           reflexivity. }
+         { rewrite (IHs2 F D Es Et); eauto with cset.
+           reflexivity. }
+  - rewrite (IHs1 F D Es Et); eauto with cset.
+    rewrite (IHs2 F D Es Et); eauto with cset.
+    reflexivity.
   - case_eq (exp_eval (to_partial (to_total (combineEnv D Es Et))) e); intros;
     case_eq (exp_eval (to_partial (to_total (combineEnv D Es Et))) e0); intros.
     + pose proof (exp_combineenv_eqr' e D Es Et (Some v)).
@@ -224,35 +210,28 @@ Proof.
          rewrite H2, H5, H4, H7; eauto; intuition.
        }
     + pose proof (exp_combineenv_eqr' e D Es Et (Some v)).
-      assert (agree_on eq (Exp.freeVars e ∩ D) Es Et).
-      * setSubst2 H.
-      * destruct H2; eauto. specialize (H2 H0).
-        pose proof (exp_combineenv_eqr' e0 D Es Et None).
-        assert (agree_on eq (Exp.freeVars e0 ∩ D) Es Et).
-        { setSubst2 H. }
-        { destruct H5; eauto. specialize (H5 H1).
-          unfold smt_eval.
-          rewrite H0, H1, H2, H5; intuition.
-        }
+      assert (agree_on eq (Exp.freeVars e ∩ D) Es Et) by eauto with cset.
+      destruct H2; eauto. specialize (H2 H0).
+      pose proof (exp_combineenv_eqr' e0 D Es Et None).
+      assert (agree_on eq (Exp.freeVars e0 ∩ D) Es Et) by eauto with cset.
+      destruct H5; eauto. specialize (H5 H1).
+      unfold smt_eval.
+      rewrite H0, H1, H2, H5; intuition.
     + pose proof (exp_combineenv_eqr' e D Es Et None).
-      assert (agree_on eq (Exp.freeVars e ∩ D) Es Et).
-      * setSubst2 H.
-      * destruct H2; eauto. specialize (H2 H0).
-        pose proof (exp_combineenv_eqr' e0 D Es Et (Some v)).
-        destruct H5.
-        { setSubst2 H. }
-        { specialize (H5 H1).
+      assert (agree_on eq (Exp.freeVars e ∩ D) Es Et) by eauto with cset.
+      destruct H2; eauto. specialize (H2 H0).
+      pose proof (exp_combineenv_eqr' e0 D Es Et (Some v)).
+      destruct H5; eauto with cset.
+      { specialize (H5 H1).
         unfold smt_eval.
         rewrite H0, H1, H2, H5.
         intuition. }
     + pose proof (exp_combineenv_eqr' e D Es Et None).
-      assert (agree_on eq (Exp.freeVars e ∩ D) Es Et).
-      * setSubst2 H.
-      * destruct H2; eauto. specialize (H2 H0).
-        pose proof (exp_combineenv_eqr' e0 D Es Et None).
-        destruct H5.
-        { setSubst2 H. }
-        { unfold smt_eval. rewrite H0, H1, H2, H5; eauto.
+      assert (agree_on eq (Exp.freeVars e ∩ D) Es Et) by eauto with cset.
+      destruct H2; eauto. specialize (H2 H0).
+      pose proof (exp_combineenv_eqr' e0 D Es Et None).
+      destruct H5; eauto with cset.
+      { unfold smt_eval. rewrite H0, H1, H2, H5; eauto.
         intuition. }
   -  simpl. unfold labInc. destruct p.
      (* TODO: Make Lemma *)
@@ -264,25 +243,16 @@ Proof.
          pose proof (exp_combineenv_eqr' a D Es Et (exp_eval (to_partial (to_total Et)) a)).
          pose proof (exp_combineenv_eqr' a D Es Et
                                          (exp_eval (to_partial (to_total (combineEnv D Es Et))) a)).
-         destruct H0.
-         { setSubst2 H. eapply list_union_start_swap; cset_tac; eauto. }
-         { destruct H1.
-           - setSubst2 H. eapply list_union_start_swap; cset_tac; eauto.
+         simpl in *. rewrite list_union_start_swap in H.
+         destruct H0; eauto with cset.
+         { destruct H1; eauto with cset.
            - clear H3. clear H0.
              unfold smt_eval at 1. rewrite H1; eauto.
              unfold smt_eval at 2.
              destruct (exp_eval (to_partial (to_total (combineEnv D Es Et))) a);
                f_equal.
-             + erewrite (IHa n _ D Es Et); eauto.
-               eapply (agree_on_incl (lv:=freeVars (funcApp (LabI n) (a::a0)) ∩ D) ); eauto.
-               cset_tac; eauto.
-               simpl. eapply list_union_start_swap.
-               cset_tac; eauto.
-             + erewrite (IHa n _ D Es Et); eauto.
-               eapply (agree_on_incl (lv:= (freeVars (funcApp (LabI n) (a::a0)) ∩ D))) ; eauto.
-               cset_tac; eauto; simpl.
-               eapply list_union_start_swap.
-               cset_tac; eauto.
+             + erewrite (IHa n _ D Es Et); eauto with cset.
+             + erewrite (IHa n _ D Es Et); eauto with cset.
          }
      + rewrite H0; intuition.
     Grab Existential Variables.
