TransVal/NoFun.v
@@ -1,0 +1,101 @@
+Require Import IL.
+
+Inductive noFun : stmt->Prop :=
+|noFunLet x e s :
+   noFun s
+   -> noFun (stmtLet x e s)
+|noFunIf e s t :
+   noFun s
+   -> noFun t
+   -> noFun (stmtIf e s t)
+|noFunCall l Y :
+   noFun (stmtApp l Y)
+|noFunExp e :
+   noFun (stmtReturn e).
+
+
+Inductive Terminates :F.state -> F.state -> Prop :=
+|TerminatesReturn L E e v:
+   exp_eval E e = ⎣v⎦
+   -> Terminates (L, E, stmtReturn e)   (L  , E , stmtReturn e)
+|TerminatesApp L E f x vl:
+   omap (exp_eval E) x = ⎣vl⎦
+   -> Terminates (L, E, stmtApp f x) (L, E, stmtApp f x)
+|TerminatesStep L E s L'  E' s'  L'' E'' s''  a:
+   F.step (L, E, s) a (L', E', s')
+   -> Terminates (L', E', s') (L'', E'', s'')
+   ->  (forall f xl, s <> stmtApp f xl)
+   -> Terminates (L,E,s) (L'', E'', s'') .
+
+Inductive Crash : F.state -> F.state -> Prop :=
+|CrashApp L E f Y:
+   omap (exp_eval E) Y = None
+   -> Crash (L, E, stmtApp f Y) (L, E, stmtApp f Y)
+|CrashBase L E s :
+   ( forall f el, s <> stmtApp f el)
+   ->  normal2 F.step (L, E, s)
+   -> state_result (L,E,s) = None
+   -> Crash (L, E,s) (L,E,s)
+|CrashStep L E s sigma' sigma'' a:
+   F.step (L, E, s) a sigma'
+   ->  (forall f xl, s <> stmtApp f xl)
+   -> Crash sigma' sigma''
+   -> Crash (L,E,s) sigma''.
+
+(** Lemma 2 of the thesis
+It is decidable wether program leaf crashes or leaf terminates **)
+Lemma noFun_impl_term_crash :
+  forall E s,
+    noFun s
+    ->  exists E' s',
+    forall L,
+      Terminates (L, E, s)(L, E', s') \/ Crash (L, E, s) (L, E', s').
+
+Proof.
+  intros E s noFun_s; general induction noFun_s.
+  -  case_eq (exp_eval E e); intros.
+     + destruct (IHnoFun_s (E[x<- Some v])) as [E' [s' termcrash]].
+       exists E'; exists s'; intros.
+       destruct (termcrash L) as [ term | crash].
+       * left. econstructor; eauto.
+         { econstructor; eauto. }
+         { intros. hnf; isabsurd. }
+       * right. econstructor; eauto; try  econstructor; eauto; intros; isabsurd.
+     + exists E; exists (stmtLet x e s); intros.
+       right. econstructor; eauto; intros; try hnf; try isabsurd.
+       intros. unfold reducible2 in H0. destruct H0 as [y [σ' H0]].
+       isabsurd.
+  - case_eq (exp_eval E e); intros.
+    + case_eq (val2bool v); intros.
+      * destruct (IHnoFun_s1 E) as [E' [s' termcrash]].
+        exists E'; exists s'; intros.
+        destruct (termcrash L) as [term | crash].
+        { left. econstructor; eauto.
+          - econstructor; eauto.
+          - hnf; intros; isabsurd. }
+        { right. econstructor; eauto. econstructor; eauto.
+          intros; isabsurd. }
+      * destruct (IHnoFun_s2 E) as [E' [s' termcrash]];
+          exists E'; exists s'; intros.
+        destruct (termcrash L) as [ term | crash ].
+        { left. econstructor; eauto.
+          - econstructor; eauto.
+          - hnf; intros; isabsurd. }
+        { right. econstructor; eauto. econstructor; eauto.
+          intros; isabsurd. }
+    +  exists E; exists (stmtIf e s t).
+       right. econstructor; eauto; intros; try hnf; try isabsurd.
+       intros. unfold reducible2 in H0. destruct H0 as [y [σ' H0]].
+       isabsurd.
+  - case_eq (omap (exp_eval E) Y); intros.
+    + exists E; exists (stmtApp l Y); left; econstructor; eauto.
+    + exists E; exists (stmtApp l Y); right.
+      econstructor; eauto; intros; try hnf; try isabsurd.
+  - case_eq (exp_eval E e).
+    + exists E; exists (stmtReturn e).
+      left; econstructor; eauto.
+    + exists E; exists (stmtReturn e). right.
+      econstructor; eauto; intros; try hnf; try isabsurd.
+      intros. unfold reducible2 in H0. destruct H0.
+      destruct H0. inversion H0.
+Qed.
